\documentclass[12pt]{article}
\usepackage{fullpage}
\usepackage{titlesec}
\usepackage{tikz}
\usepackage{amsfonts,amssymb}
\usepackage{amsmath}
\usepackage{comment}
\usetikzlibrary{automata, positioning}

\input ../libraries/mac.tex
\input ../libraries/mathmac.tex

\begin{document}
\pagestyle{plain}
\titleformat{\subsection}[runin]
  {\normalfont\large\bfseries}{\thesubsection}{1em}{}
\titleformat{\subsubsection}[runin]
  {\bfseries}{}{1em}{}

\title{Homework 6}
\author{Brooke Fugate, Michael O'Connor, Rohan Shah}
\date{}

\maketitle

\section*{Problem B4}
\subsection*{A(0, x)} 
$$A(0, x) = x + 1$$
\subsection*{A(1, x)}
$$A(1, 0) = A(0, 1) = 2$$
$$A(1, x + 1) = A(0, A(1, x)) = A(0, x + 2) = x + 3 = (x + 1) +2$$
\subsection*{A(2, x)} 
$$A(2, 0) = A(1, 1) = A(0, A(1, 0) = A(0, 2) = 3$$
$$A(2, x + 1) = A(1, A(2, x)) = A(1, 2x + 3) = (2x + 3) +2 = 2x + 5 = 2(x + 1) + 3$$
\subsection*{A(3, x)} 
$$A(3, 0) = A(2, 1) = A(1, A(2, 0) = A(1, 3) = 5$$
$$A(3, x + 1) = A(2, A(3, x)) = A(2, 2^{x + 3} - 3) = 2*(2^{x+3} - 3)  + 3 = 2^{x + 1 + 3} - 3$$
\subsection*{A(4, x)} 
$$A(4, 0) = A(3, 1) = 2^{1 + 3} - 3 = 2^4 -3 = 13$$
$$A(4, x + 1) = A(3, A(4, x)) = A(3,  \supexpo{2}{2}{x + 3}\> - 3) = (2^{\supexpo{2}{2}{x + 3}\>} - 3 = \supexpo{2}{2}{x + 1 + 3}\> - 3$$
\end{document}
