\documentclass[12pt]{article}
\usepackage{fullpage}
\usepackage{titlesec}
\usepackage{tikz}
\usepackage{amsfonts,amssymb}
\usepackage{amsmath}
\usepackage{comment}
\usetikzlibrary{automata, positioning}

\input ../libraries/mac.tex
\input ../libraries/mathmac.tex

\begin{document}
\pagestyle{plain}
\titleformat{\subsection}[runin]
  {\normalfont\large\bfseries}{\thesubsection}{1em}{}

\title{Homework 5}
\author{Brooke Fugate, Michael O'Connor, Rohan Shah}
\date{}

\maketitle

\section*{Problem B3}
Given a context-free language $L$ and a regular language $R$, prove that
$L\cap R$ is context-free. Proof by construction of a CFG $G_2$ such that
$L(G_2) = L\cap R$. Let $G = (V,\Sigma,P,S)$ be a CFG in Chomsky normal form
such that $L(G) = L$ and $N = V - \Sigma$ be the set of nonterminals in $G$.
Let $D = (Q,\Sigma, \delta, q_0, F)$ be a DFA such that $L(D) = R$.
Let $G_2 = (V',\Sigma,P',S_0)$ be a CFG where $N' = V' - \Sigma$ be the set of
nonterminals in $G_2$ where $N' = Q\times N\times Q \cup \{S_0\}$ and
productions in $P'$ are defined by the following properties:
\begin{itemize}
\item $(S_0 \rightarrow (q_0,S,f)) \in P'$ for every $f \in F$
\item $(S_0 \rightarrow \epsilon) \in P' \iff (S\rightarrow \epsilon) \in P$ and
$q_0 \in F$
\item $((p,A,\delta(p,a)) \rightarrow a) \in P' \iff (A \rightarrow a) \in P$
for all $a \in \Sigma$, all $A \in N$, and all $p \in Q$.
\item $((p,A,s) \rightarrow (p,B,q)(q,C,s)) \in P' \iff (A \rightarrow BC)\in P$
for all $p,q,s \in Q$ and all $A,B,C \in N$
\end{itemize}
\textbf{Claim: } For all $p,q\in Q$, all $A\in N$, all $w\in \Sigma^+$,
and all $n\ge 1$
$$(p,A,q) \underset{lm}{\overset{n}{\Longrightarrow}}_{G_2} w
\iff A \underset{lm}{\overset{n}{\Longrightarrow}}_{G} w
\text{ and } \delta^*(p,w) = q$$
\textbf{Case: } $(p,A,q) \underset{lm}{\overset{n}{\Longrightarrow}}_{G_2} w
\implies A \underset{lm}{\overset{n}{\Longrightarrow}}_{G} w
\text{ and } \delta^*(p,w) = q$
\newline \textbf{Proof: } By induction on $n$
\newline \textbf{Base Case: } $n = 1$.
\medskip \newline
So given that
$$((p,A,q) \rightarrow a) \in P' \text{ for } a\in \Sigma$$
We need to prove that
$$ (A \rightarrow a) \in P \text{ and } \delta(p,a) = q$$
Which we have immediately from our above construction of $P'$ where
$$((p,A,\delta(p,a)) \rightarrow a) \in P' \implies
((p,A,q) \rightarrow a) \in P' \text{ where } q=\delta(p,a) \text{ and }
(A\rightarrow a) \in P$$
\newline \textbf{Inductive Case: } $n = n+1$.
\newline \textbf{Induction Hypothesis: }
$(p,A,q) \underset{lm}{\overset{n}{\Longrightarrow}}_{G_2} w
\implies A \underset{lm}{\overset{n}{\Longrightarrow}}_{G} w
\text{ and } \delta^*(p,w) = q$.
\medskip \newline
So given that
$$(p,A,q) \underset{lm}{\overset{n+1}{\Longrightarrow}}_{G_2} w$$
We need to prove that
$$A \underset{lm}{\overset{n+1}{\Longrightarrow}}_{G} w
\text{ and } \delta^*(p,w) = q$$
From our construction of $G_2$ above we have that
$$(p,A,q) \rightarrow (p,B,s)(s,C,q)
\underset{lm}{\overset{n}{\Longrightarrow}}_{G} w$$
Let $w=uv$ where $u,v\in \Sigma^*$ then we have
$$ (p,A,q) \rightarrow (p,B,s)(s,C,q)
\underset{lm}{\overset{n_1}{\Longrightarrow}}_{G} u(s,C,q)
\underset{lm}{\overset{n_2}{\Longrightarrow}}_{G} uv = w
\text{ where } n_1,n_2 \le n $$
Then by the induction hypothesis we have that
$$B \underset{lm}{\overset{n_1}{\Longrightarrow}}_{G} u
\text{ and } \delta^*(p,u) = s$$
$$C \underset{lm}{\overset{n_2}{\Longrightarrow}}_{G} v
\text{ and } \delta^*(s,v) = q$$
And by construction we have
$$A\rightarrow BC \in P$$
So we have that
$$A \rightarrow BC \underset{lm}{\overset{n_1}{\Longrightarrow}}_{G} uC
\underset{lm}{\overset{n_1}{\Longrightarrow}}_{G} uv
\text{ and } \delta^*(\delta^*(p,u),v) = q$$
which is equivalent to
$$A \underset{lm}{\overset{n+1}{\Longrightarrow}}_{G} w
\text{ and } \delta^*(p,w) = q$$
which is what we are trying to prove.
\medskip \newline
\textbf{Case: } $A \underset{lm}{\overset{n}{\Longrightarrow}}_{G} w
\text{ and } \delta^*(p,w) = q \implies
(p,A,q) \underset{lm}{\overset{n}{\Longrightarrow}}_{G_2} w$
\newline \textbf{Proof: } By induction on $n$
\newline \textbf{Base Case: } $n = 1$.
\medskip \newline
So given that
$$ (A \rightarrow a) \in P \text{ and } \delta(p,a) = q$$
We need to prove that
$$((p,A,q) \rightarrow a) \in P' \text{ for } a\in \Sigma$$
By construction we have that
$$(A \rightarrow a) \in P \implies ((p,A,\delta(p,a)) \rightarrow a) \in P'$$
and by substituion we have
$$((p,A,q) \rightarrow a) \in P'$$
so the base case is proven trivially.
\medskip \newline
\textbf{Inductive Case: } $n = n+1$.
\newline \textbf{Induction Hypothesis: }
$A \underset{lm}{\overset{n}{\Longrightarrow}}_{G} w
\text{ and } \delta^*(p,w) = q \implies
(p,A,q) \underset{lm}{\overset{n}{\Longrightarrow}}_{G_2} w$
\medskip \newline
So given that
$$A \underset{lm}{\overset{n+1}{\Longrightarrow}}_{G} w
\text{ and } \delta^*(p,w) = q$$
We need to prove that
$$(p,A,q) \underset{lm}{\overset{n+1}{\Longrightarrow}}_{G_2} w$$
Since $G$ is in Chomskey normal form we have that
$$A \rightarrow BC \underset{lm}{\overset{n}{\Longrightarrow}}_{G} w$$
Let $w =uv$ for $u,v\in \Sigma^*$, then we have
$$A \rightarrow BC \underset{lm}{\overset{n_1}{\Longrightarrow}}_{G} uC
\underset{lm}{\overset{n_2}{\Longrightarrow}}_{G} uv
\text{ where } n_1,n_2\le n$$
So we have
$$B \underset{lm}{\overset{n_1}{\Longrightarrow}}_{G} u
\text{ and } \exists s\in Q,\ \delta^*(p,u) = s$$
$$C \underset{lm}{\overset{n_2}{\Longrightarrow}}_{G} v
\text{ and } \exists q\in Q,\ \delta^*(s,u) = q$$
So by the induction hypothesis we have
$$(p,B,s) \underset{lm}{\overset{n}{\Longrightarrow}}_{G_2} u$$
$$(s,C,q) \underset{lm}{\overset{n}{\Longrightarrow}}_{G_2} v$$
and by construction given that we have (from above) that
$$A \rightarrow BC \in P$$
we have
$$(p,A,q) \rightarrow (p,B,s)(s,C,q) \in P'$$
so by substitution we have
$$(p,A,q) \rightarrow (p,B,s)(s,C,q)
\underset{lm}{\overset{n_1}{\Longrightarrow}}_{G_2} u(s,C,q)
\underset{lm}{\overset{n_2}{\Longrightarrow}}_{G_2} uv$$
which is equivalent to
$$(p,A,q) \underset{lm}{\overset{n+1}{\Longrightarrow}}_{G_2} w$$
which is what we are trying to prove. So our claim is fully proven.
We can now show that $L(G_2) = L\cap R$. By definition
$L(G_2) = \{w \in \Sigma^* \mid S_0 \overset{+}{\Longrightarrow} w\}$,
$L = L(G) = \{w \in \Sigma^* \mid S \overset{+}{\Longrightarrow} w\}$, and
$R = L(D) = \{w \in \Sigma^* \mid \delta^*(q_0,w) \in F\}$. By our
construction of $G_2$ we have that
$$(S_0 \rightarrow (q_0,S,f)) \in P' \text{ for every } f \in F$$
and by our above claim we know that
$$(q_0,S,f) \underset{lm}{\overset{n}{\Longrightarrow}}_{G_2} w \iff
S \underset{lm}{\overset{n}{\Longrightarrow}}_{G} w
\text{ and } \delta^*(q_0,w) = f \text{ where } f\in F$$
Therefore it is immediate that
$$ S_0 \overset{+}{\Longrightarrow}_{G_2} w \iff
S \overset{+}{\Longrightarrow}_{G} w \text{ and } \delta^*(q_0,w) \in F$$
thus $L(G_2) = L\cap R$ which implies that the language $L\cap R$ is
context-free.

\end{document}
